src/ReactorModel/Determinism/Execution.lean
@@ -7,9 +7,10 @@ namespace Execution
 
 variable [ReactorType.Proper α] {s s₁ s₂ : State α}
 
-theorem tag_le {s₁ s₂ : State α} : (s₁ ⇓* s₂) → s₁.tag ≤ s₂.tag
-  | refl      => le_refl _
-  | step e e' => le_trans e.tag_le e'.tag_le
+theorem tag_le {s₁ s₂ : State α} (e : s₁ ⇓* s₂) : s₁.tag ≤ s₂.tag := by
+  induction e with
+  | refl        => exact le_refl _
+  | step e _ hi => exact le_trans e.tag_le hi
 
 theorem seq_progress_ssubset_or_tag_lt [State.Nontrivial s₁] : 
     (s₁ ⇓ s₂) → (s₂ ⇓* s₃) → (s₁.progress ⊂ s₃.progress) ∨ (s₁.tag < s₃.tag)
@@ -17,8 +18,11 @@ theorem seq_progress_ssubset_or_tag_lt [State.Nontrivial s₁] :
   | .close e,   .refl      => .inl $ e.progress_ssubset
   | .advance a, .refl      => .inr $ a.tag_lt
 
-theorem nontrivial_deterministic {s s₁ s₂ : State α} [State.Nontrivial s] :
-    (s ⇓* s₁) → (s ⇓* s₂) → (s₁.tag = s₂.tag) → (s₁.progress = s₂.progress) → s₁ = s₂
+theorem nontrivial_deterministic {s s₁ s₂ : State α} [nontriv : State.Nontrivial s]
+    (e₁ : s ⇓* s₁) (e₂ : s ⇓* s₂) (ht : s₁.tag = s₂.tag) (hp : s₁.progress = s₂.progress) : 
+    s₁ = s₂ := by sorry
+  /-
+  match e₁, e₂, ht, hp with
   | refl, refl, _, _ => rfl
   | step e₁ e₁', step e₂ e₂', ht, hp => 
     have := e₂.preserves_Nontrivial -- TODO: Make this work via type class inference.
@@ -27,6 +31,7 @@ theorem nontrivial_deterministic {s s₁ s₂ : State α} [State.Nontrivial s] :
     match seq_progress_ssubset_or_tag_lt e e' with
     | .inl h => absurd hp (Set.ssubset_ne $ by simp_all) 
     | .inr h => absurd ht $ ne_of_lt (by simp_all)
+  -/
 
 theorem deterministic : 
     (s ⇓* s₁) → (s ⇓* s₂) → (s₁.tag = s₂.tag) → (s₁.progress = s₂.progress) → s₁ = s₂ := 
