src/ReactorModel/Execution/Progress.lean
@@ -1,0 +1,25 @@
+import ReactorModel.Execution.Trace
+
+open ReactorType
+
+-- TODO: Move the Determinism folder into the Execution folder.
+--       Perhaps also rename it to Theorems, as it contains many lemmas which aren't only relevant
+--       to proving determinism.
+
+namespace Execution
+
+variable [Proper α]
+
+structure State.Terminal (s : State α) : Prop where
+  closed  : s.Closed
+  no_next : ∀ g, ¬s.NextTag g
+
+-- A reactor has the progress property, if from any nonterminal state based at that reactor, we can 
+-- perform an execution step.
+def Progress (rtr : α) : Prop :=
+  ∀ {s : State α}, (s.rtr = rtr) → ¬s.Terminal → (∃ s', s ⇓ s')    
+
+theorem Progress.iff_deps_acyclic {rtr : α} : (Progress rtr) ↔ (Dependency.Acyclic rtr) :=
+  sorry
+
+end Execution
